cp, linking dice*

pulse/pulse2rust/dpe/src/l0core.rs
@@ -1,3 +1,10 @@
+use once_cell::sync::Lazy;
+pub static L0: Lazy<super::l0core_gen::l0> =
+    Lazy::new(|| unsafe { super::l0core_gen::l0::new("l0.so").unwrap() });
+
+pub type deviceIDCSR_ingredients_t = super::l0core_gen::L0Core_deviceIDCSR_ingredients_t;
+pub type aliasKeyCRT_ingredients_t = super::l0core_gen::L0Core_aliasKeyCRT_ingredients_t;
+
 pub fn l0(
     cdi: &mut [u8],
     fwid: &mut [u8],
@@ -5,8 +12,8 @@ pub fn l0(
     deviceID_label: &mut [u8],
     aliasKey_label_len: u32,
     aliasKey_label: &mut [u8],
-    deviceIDCSR_ingredients: super::l0types::deviceIDCSR_ingredients_t,
-    aliasKeyCRT_ingredients: super::l0types::aliasKeyCRT_ingredients_t,
+    deviceIDCSR_ingredients: super::l0core_gen::L0Core_deviceIDCSR_ingredients_t,
+    aliasKeyCRT_ingredients: super::l0core_gen::L0Core_aliasKeyCRT_ingredients_t,
     deviceID_pub: &mut [u8],
     aliasKey_pub: &mut [u8],
     aliasKey_priv: &mut [u8],
@@ -24,4 +31,23 @@ pub fn l0(
     deviceIDCSR_buf_repr: (),
     aliasKeyCRT_buf_repr: (),
 ) {
+    unsafe {
+        L0.L0Core_l0(
+            cdi.as_mut_ptr(),
+            fwid.as_mut_ptr(),
+            deviceID_label_len,
+            deviceID_label.as_mut_ptr(),
+            aliasKey_label_len,
+            aliasKey_label.as_mut_ptr(),
+            deviceIDCSR_ingredients,
+            aliasKeyCRT_ingredients,
+            deviceID_pub.as_mut_ptr(),
+            aliasKey_pub.as_mut_ptr(),
+            aliasKey_priv.as_mut_ptr(),
+            deviceIDCSR_len,
+            deviceIDCSR_buf.as_mut_ptr(),
+            aliasKeyCRT_len,
+            aliasKeyCRT_buf.as_mut_ptr(),
+        )
+    }
 }
