pulse/pulse2rust/dpe/src/l0types.rs
@@ -4,44 +4,14 @@
 ////
 ////
 
-pub struct character_string_t {
-    pub fst: u32,
-    pub snd: std::vec::Vec<char>,
-}
-pub struct octet_string_t {
-    pub len: u32,
-    pub s: std::vec::Vec<char>,
-}
-pub struct deviceIDCSR_ingredients_t {
-    pub ku: i32,
-    pub version: i32,
-    pub s_common: super::l0types::character_string_t,
-    pub s_org: super::l0types::character_string_t,
-    pub s_country: super::l0types::character_string_t,
-}
-pub struct aliasKeyCRT_ingredients_t {
-    pub version1: i32,
-    pub serialNumber: super::l0types::octet_string_t,
-    pub i_common: super::l0types::character_string_t,
-    pub i_org: super::l0types::character_string_t,
-    pub i_country: super::l0types::character_string_t,
-    pub notBefore: std::vec::Vec<char>,
-    pub notAfter: std::vec::Vec<char>,
-    pub s_common1: super::l0types::character_string_t,
-    pub s_org1: super::l0types::character_string_t,
-    pub s_country1: super::l0types::character_string_t,
-    pub ku1: i32,
-    pub l0_version: i32,
-}
 pub struct l0_record_t {
     pub fwid: std::vec::Vec<u8>,
     pub deviceID_label_len: u32,
     pub deviceID_label: std::vec::Vec<u8>,
     pub aliasKey_label_len: u32,
     pub aliasKey_label: std::vec::Vec<u8>,
-    pub deviceIDCSR_ingredients: super::l0types::deviceIDCSR_ingredients_t,
-    pub aliasKeyCRT_ingredients: super::l0types::aliasKeyCRT_ingredients_t,
+    pub deviceIDCSR_ingredients: super::l0core::deviceIDCSR_ingredients_t,
+    pub aliasKeyCRT_ingredients: super::l0core::aliasKeyCRT_ingredients_t,
     pub deviceIDCSR_len: u32,
     pub aliasKeyCRT_len: u32,
 }
-
