pulse/share/pulse/examples/dice/external/l0/L0Core.fsti
@@ -17,12 +17,57 @@
 module L0Core
 
 open Pulse.Lib.Pervasives
-open L0Types
 
 module G = FStar.Ghost
 module U8 = FStar.UInt8
 module U32 = FStar.UInt32
+module I32 = FStar.Int32
 module A = Pulse.Lib.Array
+
+noeq
+type character_string_t = {
+  fst : U32.t;
+  snd : FStar.Bytes.bytes;
+}
+
+noeq
+type octet_string_t = {
+  len : U32.t;
+  s : FStar.Bytes.bytes;
+}
+
+noeq
+type deviceIDCSR_ingredients_t = {
+  ku        : I32.t;
+  version   : I32.t;
+  s_common  : character_string_t;
+  s_org     : character_string_t;
+  s_country : character_string_t;
+}
+
+noeq
+type aliasKeyCRT_ingredients_t = {
+  version       : I32.t;
+  serialNumber  : octet_string_t;
+  i_common      : character_string_t;
+  i_org         : character_string_t;
+  i_country     : character_string_t;
+  notBefore     : FStar.Bytes.bytes;
+  notAfter      : FStar.Bytes.bytes;
+  s_common      : character_string_t;
+  s_org         : character_string_t;
+  s_country     : character_string_t;
+  ku            : I32.t;
+  l0_version    : I32.t;
+}
+
+val valid_hkdf_lbl_len (n:U32.t) : prop
+val valid_deviceIDCSR_ingredients
+  (deviceIDCSR_ingredients:deviceIDCSR_ingredients_t)
+  (deviceIDCSR_len:U32.t) : prop
+val valid_aliasKeyCRT_ingredients
+  (aliasKeyCRT_ingredients:aliasKeyCRT_ingredients_t)
+  (aliasKeyCRT_len:U32.t) : prop
 
 val l0_post
   (cdi_repr fwid_repr:Seq.seq U8.t)
