pulse/pulse2rust/dpe/rust.Dockerfile
@@ -7,4 +7,6 @@ RUN rustup component add rustfmt
 RUN cargo install bindgen-cli
 ADD _output/*.h .
 ADD krmllib.h .
+ADD compat.h .
 RUN bindgen -o evercrypt_gen.rs --allowlist-file '.*EverCrypt.*' bindings.h --dynamic-loading "evercrypt" --dynamic-link-require-all
+RUN bindgen -o l0core_gen.rs --allowlist-file '.*L0Core.*' bindings.h --dynamic-loading "l0" --dynamic-link-require-all
